semantics/proofs/typeSoundInvariantsScript.sml
@@ -8,8 +8,7 @@ val _ = numLib.prefer_num();
 
 val _ = new_theory "typeSoundInvariants"
 
-(* Type system for values, evaluation contexts, and the small-step sematnics'
- * states. The invariant that is used for type soundness. *)
+(* Type system for values. The invariant that is used for type soundness. *)
 
 (*open import Pervasives*)
 (*open import Lib*)
